ConNF.lean
@@ -23,6 +23,7 @@ import ConNF.Counting.CountSupportOrbit
 import ConNF.Counting.Recode
 import ConNF.Counting.Twist
 import ConNF.External.Basic
+import ConNF.External.Counting
 import ConNF.External.WellOrder
 import ConNF.FOA.BaseAction
 import ConNF.FOA.BaseApprox
