ConNF/External/Counting.lean
@@ -1,0 +1,36 @@
+import ConNF.External.Basic
+
+/-!
+# New file
+
+In this file...
+
+## Main declarations
+
+* `ConNF.foo`: Something new.
+-/
+
+noncomputable section
+universe u
+
+open Cardinal Ordinal ConNF.TSet
+
+namespace ConNF
+
+variable [Params.{u}] {α β γ δ ε ζ : Λ} (hβ : (β : TypeIndex) < α) (hγ : (γ : TypeIndex) < β)
+  (hδ : (δ : TypeIndex) < γ) (hε : (ε : TypeIndex) < δ) (hζ : (ζ : TypeIndex) < ε)
+
+/-- The set `{z ∪ {a} | z ∈ x}`. -/
+def insert (x : TSet α) : TSet α :=
+  sorry
+
+def cardinalNat (n : ℕ) : TSet α :=
+  (TSet.exists_cardinalOne hβ hγ).choose
+
+@[simp]
+theorem mem_cardinalNat_iff (n : ℕ) :
+    ∀ a : TSet β, a ∈' cardinalNat hβ hγ n ↔
+    ∃ s : Finset (TSet γ), s.card = n ∧ ∀ b : TSet γ, b ∈' a ↔ b ∈ s :=
+  sorry
+
+end ConNF
